coq/Puiseux_base.v
@@ -1,4 +1,4 @@
-(* $Id: Puiseux_base.v,v 1.24 2013-06-17 13:58:28 deraugla Exp $ *)
+(* $Id: Puiseux_base.v,v 1.25 2013-06-17 15:23:06 deraugla Exp $ *)
 
 (* Most of notations are Robert Walker's ones *)
 
@@ -45,14 +45,14 @@ Record term α := { coeff : α; power : Q }.
 Axiom series_head : ∀ α, series (term α) → series (term α).
 
 Definition den_divides_comden comden p :=
-  (' Qden p | (Z.of_nat comden * Qnum p))%Z.
+  (' Qden p | (Zpos comden * Qnum p))%Z.
 
 Definition pow_den_div_com_den α comden (t : term α) :=
   den_divides_comden comden (power t).
 
 Record puiseux_series α :=
   { ps_terms : series (term α);
-    ps_comden : nat;
+    ps_comden : positive;
     ps_prop : series_forall (pow_den_div_com_den ps_comden) ps_terms }.
 
 Definition valuation α (ps : puiseux_series α) :=
